src/compiler/meta/OCL_compiler_parser_UML.thy
@@ -284,8 +284,8 @@ definition "i_of_ocl_ass_class a b = rec_ocl_ass_class
     (i_of_ocl_association a b (K i_of_unit))
     (i_of_ocl_class_raw a b (K i_of_unit)))"
 
-definition "i_of_ocl_enum a b = rec_ocl_enum
-  (ap2 a (b \<open>OclEnumSynonym\<close>)
+definition "i_of_ocl_class_synonym a b = rec_ocl_class_synonym
+  (ap2 a (b \<open>OclClassSynonym\<close>)
     (i_of_string a b)
     (i_of_ocl_ty a b))
   (ap2 a (b \<open>OclEnum\<close>)
@@ -317,6 +317,6 @@ lemmas [code] =
   i_of.i_of_ocl_class_def
   i_of.i_of_ocl_class_raw_def
   i_of.i_of_ocl_ass_class_def
-  i_of.i_of_ocl_enum_def
+  i_of.i_of_ocl_class_synonym_def
 
 end
